Assumptions:
\begin{enumerate}
    \item $\varepsilon \text{ is independent from } x \text{ which gives: }\mathbb{E}[\varepsilon]=0)$
    \item $y=f(x) + \varepsilon$ \text{. Here we will simplify f=f(x)}.
    \item $f(x) \text{ is a fixed, deterministic function of } x \text{, hence }\\ \mathbb{E}[f(x)]=f(x)$
\end{enumerate}
{The mean-square error of our model can be written:}
%
%_____________________________________
%
\begin{align*}
    & \text{MSE} = \mathbb{E}[(y-\Tilde{y})^2]\\
    & = \mathbb{E}[y^2-2y\Tilde{y}+\Tilde{y}^2]\\
    & = \mathbb{E}[y^2]-2\mathbb{E}[y\Tilde{y}]+\mathbb{E}[\Tilde{y}^2]\\
\end{align*}
%
We look into each term:
\begin{equation}
\mathbb{E}[y^2]
\end{equation}
\begin{equation}
    \mathbb{E}[y\Tilde{y}]
\end{equation}
\begin{equation}
    \mathbb{E}[\Tilde{y}^2]
\end{equation}
%
%Term 1 ____________
From (1) we have:
 \begin{align*}
     & \mathbb{E}[y^2]=\mathbb{E}[(f+\varepsilon)^2]=\mathbb{E}[f^2+2f\varepsilon+\epsilon^2]\\
     & = \mathbb{E}[f^2]+\mathbb{E}[\varepsilon^2]\\
     & =  \mathbb{E}[f^2]+\sigma^2 = f^2+\sigma^2
 \end{align*}
%Term 2 _________________
From (2):
\begin{align*}
    & \mathbb{E}[y\Tilde{y}]=\mathbb{E}[y]\mathbb{E}[\Tilde{y}]
     = \mathbb{E}[f+\varepsilon]\mathbb{E}[\Tilde{y}]\\
    & =\mathbb{E}[f]\mathbb{E}[\Tilde{y}]=f\mathbb{E}[\Tilde{y}]
\end{align*}
%Term 3 _________________
We have:
\begin{align*}
    & Var[\Tilde{y}]=\mathbb{E}[(\Tilde{y}]-\mathbb{E}[\Tilde{y}])^2]\\
    & = \mathbb{E}[\Tilde{y}^2-2\Tilde{y}\mathbb{E}[\Tilde{y}]+(\mathbb{E}[\Tilde{y}])^2]\\
    & = \mathbb{E}[\Tilde{y}^2]-2\mathbb{E}[\Tilde{y}]\mathbb{E}[\Tilde{y}]+(\mathbb{E}[\Tilde{y}])^2\\
    & = \mathbb{E}[\Tilde{y}^2]-(\mathbb{E}[\Tilde{y}])^2\\
    & \implies \mathbb{E}[\Tilde{y}^2]= Var[\Tilde{y}]+(\mathbb{E}[\Tilde{y}])^2
\end{align*}
%
Put the terms together:
\begin{align*}
    & \mathbb{E}[y^2]-2\mathbb{E}[y\Tilde{y}]+\mathbb{E}[\Tilde{y}^2]\\
    & = f^2+\sigma^2-2f\mathbb{E}[\Tilde{y}]+(Var(\Tilde{y})+(\mathbb{E}[\Tilde{y}])^2)\\
    & = f^2-2f\mathbb{E}[\Tilde{y}]+(\mathbb{E}[\Tilde{y}])^2+Var(\Tilde{y})+\sigma^2\\
    & \implies \mathbb{E}[(f-\mathbb{E}[\Tilde{y}])^2]+Var(\Tilde{y})+\sigma^2
\end{align*}

First term in above expression can be approximated:
\begin{equation}
    \mathbb{E}[(f-\mathbb{E}[\Tilde{y}])^2] \simeq \frac{1}{n}\sum_{i}(y_i-\mathbb{E}[\Tilde{y}])^2 \text{ ,where } f_i\simeq y_i
\end{equation}

From (4) we have that MSE can be written:
\begin{equation}
    \mathbb{E}[(f-\mathbb{E}[\Tilde{y}])^2] \simeq \frac{1}{n}\sum_{i}(y_i-\mathbb{E}[\Tilde{y}])^2 = Bias[\Tilde{y}]
\end{equation}

Similarly, the variance can be expressed as:
\begin{align*}
    \mathbb{E}[(\Tilde{y}-\mathbb{E}[\Tilde{y}])^2]\simeq\frac{1}{n}\sum_{i}(\Tilde{y_i}-\mathbb{E}[\Tilde{y}])^2 = Var[\Tilde{y}]
\end{align*}
%___________________________________________
Setting in both the bias and variance terms into the equation we obtain:

$MSE=Bias(\Tilde{y})+Var(\Tilde{y})+\sigma^2$
\hfill\break




